@prefix rdf:	<http://www.w3.org/1999/02/22-rdf-syntax-ns#> .
@prefix core:	<http://example.org/core/> .
@prefix rdfs:	<http://www.w3.org/2000/01/rdf-schema#> .
@prefix common: <http://schema.big-iot.org/common/> .
@prefix schema:	<http://schema.org/> .
@prefix skos:	<http://www.w3.org/2004/02/skos/core#> .
@prefix owl: <http://www.w3.org/2002/07/owl#>.
@prefix ns: <http://creativecommons.org/ns#>.
@prefix ssn: <http://purl.oclc.org/NET/ssnx/ssn#>.
@prefix geo: <http://www.w3.org/2003/01/geo/wgs84_pos#>.
@prefix qudt: <http://data.qudt.org/qudt/owl/1.0.0/unit.owl#>.
@prefix dul: <http://www.loa.istc.cnr.it/ontologies/DUL.owl#>.
@prefix time: <http://www.w3.org/2006/time#>.
@prefix vann: <http://purl.org/vocab/vann/>.
@prefix dcterms: <http://purl.org/dc/terms/>.
@prefix dc: <http://purl.org/dc/elements/1.1/>.
@prefix xsd: <http://www.w3.org/2001/XMLSchema#> .
@prefix dcat: <http://www.w3.org/ns/dcat#> .
@prefix itso: <http://www.owl-ontologies.com/itso> .
@prefix pricingmodel: <http://www.owl-ontologies.com/pricingmodel> .



core: dc:contributor "Achille Zappa, NUIG, Galway"@en;
                           
            dc:description ""@en;
            dc:rights "Copyright NUIGalway, Siemens, Bosch";
            dc:title " Core Model"@en;
            dcterms:issued "2020"^^xsd:date;
            dcterms:modified "2020"^^xsd:date;
            vann:preferredNamespacePrefix "core";
            vann:preferredNamespaceUri "http://example.org/core/#";
            a owl:Ontology;
            rdfs:comment " "@en;
            rdfs:label ""^^xsd:string;
            owl:versionInfo "0.1".





##Classes

core:Categorization	rdf:type	rdfs:Class ;
	rdfs:subClassOf	schema:Thing ;
	rdf:comment	"An Hierarchy of DataOffering categories" ;
	rdf:label	"Categorization" .


core:DataOffering	rdf:type	rdfs:Class ;
	rdfs:label	"DataOffering" ;
	rdfs:comment	" DataOffering represent the ata Assets that are offered on a marketplace." ;
	rdfs:subClassOf	schema:Offer .
	
core:DataOfferingCategory	rdf:type	rdfs:Class ;
	rdfs:label	"DataOfferingCategory" ;
	rdfs:comment	"Category of an DataOffering." ;
	rdfs:subClassOf	schema:Thing .
	
core:DataOfferingQuery	rdf:type	rdfs:Class ;
	rdfs:label	"DataOfferingQuery" ;
	rdfs:comment	"Consumers discover DataOfferings they're interesting through the marketplace by providing an (DataOffering) query. The query entails a specification of the type of DataOfferings the consumer is interested in" ;
	rdfs:subClassOf	schema:Demand .
	
core:DataOfferingSubscription	rdf:type	rdfs:Class ;
	rdfs:label	"DataOfferingSubscription" ;
	rdfs:comment	"Subscription of a consumer to a specific DataOffering registered by a provider." ;
	rdfs:subClassOf	schema:Thing .
	

	
core:Provider	rdf:type	rdfs:Class ;
	rdfs:label	"Provider" ;
	rdfs:comment	"Providers register their DataOfferings on a marketplace and provides access to the offered resources via a common API." ;
	rdfs:subClassOf	schema:Thing .

core:Owner	rdf:type	rdfs:Class ;
	rdfs:label	"Owner" ;
	rdfs:comment	"The original Owner of the Data that make available via providers and provides access to the offered resources via a common API." ;
	rdfs:subClassOf	schema:Thing .	
	
core:Consumer	rdf:type	rdfs:Class ;
	rdfs:label	"Consumer" ;
	rdfs:comment	"Consumers discover and subscribe to DataOfferings of interest via api / interfaces in order to access the resources." ;
	rdfs:subClassOf	schema:Thing .
	

	
##Properties

core:hasPricingModel	rdf:type	rdf:Property ;
	rdfs:label	"hasPricingModel" ;
	rdfs:comment	"Relation between an DataOffering and the PricingModel." ;
	rdfs:domain	core:DataOffering ;
	rdfs:range 	pricingmodel:PricingModel .


core:hasCatalog	rdf:type	rdf:Property ;
	rdfs:label	"hasCatalog" ;
	rdfs:comment	"A Catalog that is described in the Data Offering." ;
	rdfs:domain	core:DataOffering ;
	rdfs:range 	dcat:Catalog .


core:serviceSpecs	rdf:type	rdf:Property ;
	rdfs:label	"serviceSpecs" ;
	rdfs:comment	"Relation between an DataService and the serviceSpecs." ;
	rdfs:domain	dcat:DataService ;
	rdfs:range 	itso:ServiceSpecs .
	

core:serviceID	rdf:type	rdf:Property ;
	rdfs:label	"serviceID" ;
	rdfs:comment	"service ID" ;
	rdfs:domain	dcat:DataService ;
	rdfs:range 	rdfs:Literal .

core:consumerId	rdf:type	rdf:Property ;
	rdfs:label	"consumerId" ;
	rdfs:comment	"Identifier on a BIG-IoT marketplace of a consumer." ;
	rdfs:domain	core:Consumer ;
	rdfs:range 	rdfs:Literal .
	
core:creative_commons	rdf:type	core:LicenseType ;
	rdfs:label	"CREATIVE_COMMONS" ;
	rdfs:comment	"Creative Commons type" ;
	skos:prefLabel	"Creative Commons" .
	

core:organizationId	rdf:type	rdf:Property ;
	rdfs:label	"organizationId" ;
	rdfs:comment	"Organization identifier." ;
	rdfs:domain	schema:Organization ;
	rdfs:range 	rdfs:Literal .
	
core:providerId	rdf:type	rdf:Property ;
	rdfs:label	"providerId" ;
	rdfs:comment	"Provider identifier." ;
	rdfs:domain	core:Provider ;
	rdfs:range 	rdfs:Literal .


core:ownerId	rdf:type	rdf:Property ;
	rdfs:label	"ownerId" ;
	rdfs:comment	"ownerId identifier." ;
	rdfs:domain	core:Owner ;
	rdfs:range 	rdfs:Literal .

	
core:isActivated	rdf:type	rdf:Property ;
	rdfs:label	"isActivated" ;
	rdfs:comment	"An DataOffering has to be activated manually on the marketplace where it is registered." ;
	rdfs:domain	core:DataOffering ;
	rdfs:range 	schema:Boolean .
	
core:isProvidedBy	rdf:type	rdf:Property ;
	rdfs:label	"isProvidedBy" ;
	rdfs:comment	"Relation between an DataOffering and the provider who registered it." ;
	owl:inverseOf core:provide ;
	rdfs:domain	core:DataOffering ;
	rdfs:range 	core:Provider .
	

	
core:isRegisteredBy	rdf:type	rdf:Property ;
	rdfs:label	"isRegisteredBy" ;
	rdfs:comment	"Relation between an DataOfferingQuery and the consumer who registered it." ;
	rdfs:domain	core:DataOfferingQuery ;
	rdfs:range 	core:Consumer .

core:isOwnedBy	rdf:type	rdf:Property ;
	rdfs:label	"isOwnedBy" ;
	rdfs:comment	"Relation between an DataOffering and the owner of the datasets." ;
	owl:inverseOf core:own ;
	rdfs:domain	core:DataOffering ;
	rdfs:range 	core:Provider .
	
core:dataOffering	rdf:type	rdf:Property ;
	rdfs:label	"dataOffering" ;
	rdfs:comment	"Relation between an DataOffering and the provider who registered it." ;
	schema:inverseOf	core:isProvidedBy ;
	rdfs:domain	core:Provider ;
	rdfs:range 	core:DataOffering .
	
core:dataOfferingExpirationTime	rdf:type	rdf:Property ;
	rdfs:label	"DataOfferingExpirationTime" ;
	rdfs:comment	"Expiration time." ;
	rdfs:domain	core:DataOffering ;
	rdfs:range 	schema:DateTime .
	
core:dataOfferingId	rdf:type	rdf:Property ;
	rdfs:label	"DataOfferingId" ;
	rdfs:comment	"DataOffering identifier." ;
	rdfs:domain	core:DataOffering ;
	rdfs:range 	rdfs:Literal .
	
core:dataOfferingQuery	rdf:type	rdf:Property ;
	rdfs:label	"DataOfferingQuery" ;
	rdfs:comment	"Concepts likely to be involved in DataOfferings of a certain category." ;
	schema:inverseOf	core:isRegisteredBy ;
	rdfs:domain	core:Consumer ;
	rdfs:range 	core:DataOfferingQuery .
	


core:queryId	rdf:type	rdf:Property ;
	rdfs:label	"queryId" ;
	rdfs:comment	"DataOffering query identifier." ;
	rdfs:domain	core:Query ;
	rdfs:range 	rdfs:Literal .
	
core:refersTo	rdf:type	rdf:Property ;
	rdfs:label	"refersTo" ;
	rdfs:comment	"Concepts likely to be involved in DataOfferings of a certain category." ;
	rdfs:domain	core:DataOfferingCategory ;
	rdfs:range 	rdfs:Class .
	
core:subscribedQuery	rdf:type	rdf:Property ;
	rdfs:label	"subscribedQuery" ;
	rdfs:comment	"Relation between an DataOffering subscription and the DataOffering query that matched the DataOffering." ;
	rdfs:domain	core:DataOfferingSubscription ;
	rdfs:range 	core:DataOfferingQuery .
	
core:subscribesTo	rdf:type	rdf:Property ;
	rdfs:label	"subscribesTo" ;
	rdfs:comment	"Relation between a subscription and the DataOffering it subscribes to." ;
	rdfs:domain	core:DataOfferingSubscription ;
	rdfs:range 	core:DataOffering .
	
core:subscriptionId	rdf:type	rdf:Property ;
	rdfs:label	"subscriptionId" ;
	rdfs:comment	"Subscription identifier." ;
	rdfs:domain	core:DataOfferingSubscription ;
	rdfs:range 	rdfs:Literal .

	

	
	
core:http_get	rdf:type	core:EndpointType ;
	rdfs:label	"HTTP_GET" ;
	rdfs:comment	"HTTP GET endpoint type" ;
	skos:prefLabel	"http get" .
core:http_post	rdf:type	core:EndpointType ;
	rdfs:label	"HTTP_POST" ;
	rdfs:comment	"HTTP POST endpoint type" ;
	skos:prefLabel	"http post" .
	

	
core:expectedAnnotation	rdf:type	rdf:Property ;
	rdfs:label	"expectedAnnotation" ;
	rdfs:comment	"Annotation expected for a certain DataOffering category." ;
	rdfs:domain	core:DataOfferingCategory ;
	rdfs:range 	core:DataTypeAnnotation .
	
	


	